SEARwfun.sml
@@ -1,42 +1,55 @@
-
-fun fVar_Inst_f (pair as (P,(argl:(string * sort) list,Q))) f = 
-    let val lcs = List.foldr
-                      (fn (ns,nss) => HOLset.delete(nss,ns)
-                                      handle _ => nss) 
-                      (fvf Q) argl
-    in
-    case view_form f of
-        vPred(P0,false,args0) =>
-        if P0 = P
-        then let val venv = match_tl essps 
-                                     (List.map mk_var argl) args0
-                                     emptyvd
-             in inst_form (mk_menv venv emptyfvd) Q
-             end 
-             handle _ => f 
-        else f
-      | vConn(co,fl) => mk_conn co (List.map (fVar_Inst_f pair) fl)
-      | vPred(_,true,_) => f
-      | vQ(q,n,s,b) => 
-        (case HOLset.find (fn (n0,s0) => n0 = n) lcs of
-            NONE => mk_quant q n s (fVar_Inst_f pair b) 
-          | SOME _ =>
-            let val (n',_) = dest_var (pvariantt lcs (mk_var(n,s)))
-                val f' = rename_bound n' f 
-            in fVar_Inst_f pair f'
-            end)
-    end
-
-
 fun fVar_Inst_th (pair as (P,(argl:(string * sort) list,Q))) th = 
     let val (ct,asl,w) = dest_thm th
-        val asl' = List.map (fVar_Inst_f pair) asl
-        val w' = fVar_Inst_f pair w
+        val asl' = List.map (form.fVar_Inst_f pair) asl
+        val w' = form.fVar_Inst_f pair w
         val vs = bigunion (pair_compare String.compare sort_compare)
                           (List.map fvf (w' :: asl'))
         val newct = HOLset.union(ct,vs)
     in mk_thm (newct,asl',w')
     end
+
+
+fun fVar_Inst [pair] th = fVar_Inst_th pair th
+
+
+
+
+
+exception UNCHANGED
+ fun total f x = SOME (f x) handle e => NONE
+
+fun MAP f l = 
+   let
+     (* map2 is the version where something has changed *)
+     fun map2 A [] = List.rev A
+       | map2 A (h::t) = map2 ((f h handle e => h) :: A) t
+     (* map1 is the version to call where nothing has changed yet *)
+     fun map1 n [] = raise UNCHANGED
+       | map1 n (h::t) = 
+           case total f h of
+             SOME fh => map2 (fh::(rev $ List.take(l,n))) t
+           | NONE => map1 (n + 1) t
+   in
+     map1 0 l
+   end
+
+
+
+
+
+fun fVar_Inst_th (pair as (P,(argl:(string * sort) list,Q))) th = 
+    let val (ct,asl,w) = dest_thm th
+        val lcs = List.foldr
+                      (fn (ns,nss) => HOLset.delete(nss,ns)
+                                      handle _ => nss) 
+                      (fvf Q) argl
+        val ct' = HOLset.union(ct,lcs)
+        val aslw' = MAP (fVar_Inst_f pair) (w :: asl)
+    in mk_thm (ct',tl aslw',hd aslw')
+    end
+
+
+(*fun fVar_Inst [pair] th = fVar_Inst_th pair th*)
 
 
 fun ind_with th (ct,asl,w) = 
@@ -47,12 +60,14 @@ fun ind_with th (ct,asl,w) =
     in match_mp_tac th1 (ct,asl,w)
     end
 
+val _ = new_pred "T" [];
+val _ = new_pred "F" [];
 
 
 val _ = new_sort "set" [];
 val _ = new_sort "mem" [("A",mk_sort "set" [])];
 val _ = new_sort "rel" [("A",mk_sort "set" []),("B",mk_sort "set" [])]
-val _ = new_sort_infix "rel" "->"
+val _ = new_sort_infix "rel" "~>";
 
 val set_sort = mk_sort "set" []
 fun mem_sort A = mk_sort "mem" [A]
@@ -67,8 +82,6 @@ val _ = EqSorts := "mem" :: (!EqSorts)
 val _ = new_pred "Holds" [("R",rel_sort (mk_set "A") (mk_set "B")),
                          ("a",mem_sort (mk_set "A")),
                          ("b",mem_sort (mk_set "B"))]
-
-
 
 fun eq_sym a = 
     if mem a (!EqSorts) then 
@@ -84,54 +97,62 @@ fun eq_sym a =
     else raise ERR ("eq_sym.input sort: " ^ a ^ " does not have equality",
                     [],[],[])
 
+fun flip_fconv eqs = 
+(first_fconv (List.map (rewr_fconv o eq_sym) eqs))
 
 
-val lflip_tac =
-fconv_tac 
- (land_fconv no_conv 
- $ basic_once_fconv no_conv
- (first_fconv (List.map (rewr_fconv o eq_sym) (!EqSorts))))
+fun uex_ex f = 
+    let val th0 = iffLR $ uex_def f |> undisch
+        val c0 = concl th0
+        val ((n,s),b) = dest_exists c0
+        val th1 = assume b |> conjE1 
+        val th2 = existsI (n,s) (mk_var(n,s)) (concl th1) th1
+        val th3 = existsE (n,s) th0 th2
+    in disch f th3
+    end
 
- 
+fun uex2ex_rule th = mp (uex_ex $concl th) th
 
-val rflip_tac =
-fconv_tac 
- (rand_fconv no_conv 
- $ basic_once_fconv no_conv
- (first_fconv (List.map (rewr_fconv o eq_sym) (!EqSorts))))
+
+
+
+fun uex_expand th = dimp_mp_l2r th (uex_def $concl th)
+
+val uex_tac:tactic = fn (ct,asl,w) =>
+    let val th = uex_def w
+        val w' = snd $ dest_dimp $ concl th
+    in ([(ct,asl,w')],(sing (dimp_mp_r2l th)))
+    end
+
+
+fun ex2fsym0 name args th = th |> eqT_intro |> iffRL |> ex2fsym name args
+                               |> C mp (trueI [])
 
 
 
 val flip_tac = 
+(fconv_tac (basic_once_fconv no_conv (flip_fconv (!EqSorts))));
+
+val lflip_tac =
 fconv_tac 
- (basic_once_fconv no_conv 
-  (first_fconv (List.map (rewr_fconv o eq_sym) (!EqSorts))))
+ (land_fconv no_conv 
+ $ basic_once_fconv no_conv (flip_fconv (!EqSorts)))
+
+
+val rflip_tac =
+fconv_tac 
+ (rand_fconv no_conv 
+ $ basic_once_fconv no_conv (flip_fconv (!EqSorts)))
+
+
+val AX0 = new_ax “?A a:mem(A).T”;
+
+val Fun_def = 
+define_pred “!A B R:rel(A,B). isFun(R) <=> !x:mem(A). ?!y:mem(B). Holds(R,x,y)”;
 
 
 
-val _ = new_sort "set" [];
-val _ = new_sort "mem" [("A",mk_sort "set" [])];
-val _ = new_sort "rel" [("A",mk_sort "set" []),("B",mk_sort "set" [])]
-val _ = new_sort_infix "rel" "->"
-
-val set_sort = mk_sort "set" []
-fun mem_sort A = mk_sort "mem" [A]
-fun rel_sort A B = mk_sort "rel" [A,B]
-fun mk_set A = mk_var(A,set_sort)
-fun mk_rel R A B = mk_var(R,rel_sort A B)
-fun mk_mem a A = mk_var(a,mem_sort A)
-
-val _ = EqSorts := "rel" :: (!EqSorts)
-val _ = EqSorts := "mem" :: (!EqSorts)
-
-val _ = new_pred "Holds" [("R",rel_sort (mk_set "A") (mk_set "B")),
-                         ("a",mem_sort (mk_set "A")),
-                         ("b",mem_sort (mk_set "B"))]
-
-val Fun_def = define_pred “!A B R:rel(A,B). isFun(R) <=> !x:mem(A). ?!y:mem(B). Holds(R,x,y)”
-
-
-val Fun_expand = prove_store("Fun_expand",
+val Fun_expand = proved_th $
 e0
 (rpt strip_tac >> rw[Fun_def] >>
  rw[uex_def “?!y:mem(B).Holds(R,x,y)”] >> 
@@ -147,12 +168,367 @@ e0
  qexists_tac ‘b’ >> arw[] >> rpt strip_tac >> first_x_assum irule >>
  qexists_tac ‘x’ >> arw[])
 (form_goal
-“!A B R:A->B. isFun(R) <=>
+“!A B R:A~>B. isFun(R) <=>
  (!a.?b.Holds(R,a,b)) & 
- (!a b1 b2. Holds(R,a,b1) & Holds(R,a,b2) ==> b1 = b2)”));
+ (!a b1 b2. Holds(R,a,b1) & Holds(R,a,b2) ==> b1 = b2)”)
 
-val _ = new_fun "Eval" (mem_sort (mk_set "B"),[("R",rel_sort (mk_set "A") (mk_set "B")),
-                        ("x",mem_sort (mk_set "A"))]) 
+val EX1_mem = prove_store("EX1_mem",
+e0
+(strip_tac >> dimp_tac >> rpt strip_tac (* 2 *)
+ >-- (pop_assum (strip_assume_tac o uex_expand) >> 
+     qexists_tac ‘x’ >> arw[]) >> 
+ uex_tac >> qexists_tac ‘x’ >> arw[])
+(form_goal
+“!A. (?!x:mem(A). P(x)) <=> (?x:mem(A). P(x) & !x'. P(x') ==> x' = x)”));
 
-val Eval_def = new_ax “!A B Fn:rel(A,B). isFun(Fn) ==>!x y. Holds(Fn,x,y) <=> y = Eval(Fn,x)”
 
+(*
+val EX1 = prove_store("EX1",
+e0
+(dimp_tac >> rpt strip_tac (* 2 *)
+ >-- pop_assum (assume_tac o uex_expand))
+“(?!x. P(x)) <=> (?x. P(x) & !x'. P(x') ==> x' = x)”
+
+
+ ERR
+     ("mk_eq.the sort: set does not have equality, attempting to make equality on",
+      [set, set], [x', x], []) raised
+
+reason of why do not use a thm for def of uex
+
+*)
+
+
+fun efn (n,s) (f,th) = 
+    let 
+        val ef = mk_exists n s f
+    in
+        (ef,existsE (n,s) (assume ef) th)
+    end
+fun match_mp_tac th (ct:cont,asl:form list,w) = 
+    let
+        val (impl,gvs) = strip_forall (concl th)
+        val (hyp,conseq) = dest_imp impl
+        val (con,cvs) = strip_forall (conseq)
+        val th1 = (C specl) (undisch ((C specl) th (List.map mk_var gvs))) (List.map mk_var cvs) 
+        val (vs,evs) = partition (fn v => HOLset.member(fvf con,v)) gvs
+        val th2 = uncurry disch (itlist efn evs (hyp, th1)) 
+        val (gl,vs) = strip_forall w
+        val env = match_form (fvfl (ant th)) (fVarsl (ant th)) con gl mempty
+        val ith = inst_thm env th2
+        val gth = simple_genl (rev vs) (undisch ith)
+        val hyp = fst (dest_imp (concl ith))
+    in
+        ([(ct,asl,hyp)], sing (mp (disch hyp gth)))
+    end
+
+
+fun ir_canon th =
+  let
+    val th1 = norm (gen_all th)
+    val origl = ant th
+    val gfvs = fvfl (concl th1 :: origl) 
+    val newhyps = form_list_diff (ant th1)  origl
+    val grouped = group_hyps gfvs newhyps
+    val (cs, th2) = reconstitute' grouped th1
+  in
+    case cs of
+        [] => gen_all th2
+      | _ =>
+        let
+          val (th3,c) = conjl (rev cs) th2
+        in
+          disch c th3 |> gen_all
+        end
+  end
+
+val irule = match_mp_tac o ir_canon
+
+val Fun_expand_alt = prove_store("Fun_expand_alt",
+e0
+(rpt strip_tac >> rw[Fun_def] >>
+ rw[fVar_Inst_th ("P",
+ ([("b",mem_sort (mk_set "B"))],“Holds(R:A~>B,a,b)”)) (EX1_mem |> qspec ‘B’) |> qgen ‘a:mem(A)’])
+(form_goal
+ “!A B R:A~>B. isFun(R) <=>
+  (!a.?b.Holds(R,a,b) & 
+      !b'. Holds(R,a,b') ==> b' = b)”))
+
+val Eval_def0 = Fun_expand_alt |> iffLR 
+                               |> strip_all_and_imp
+                               |> ex2fsym0 "Eval" ["R","a"]
+                               |> qgen ‘a’
+                               |> disch_all
+                               |> gen_all
+
+val Eval_def = prove_store("Eval_def",
+e0
+(rpt strip_tac >> drule Eval_def0 >>
+ first_x_assum (qspecl_then [‘x’] strip_assume_tac) >>
+ dimp_tac >> strip_tac (*2 *)
+ >-- (first_x_assum irule >> arw[]) >>
+ arw[])
+(form_goal
+ “!A B Fn:A ~> B. isFun(Fn) ==>!x y. Holds(Fn,x,y) <=> y = Eval(Fn,x)”));
+
+
+val _ = new_sort "fun" [("A",mk_sort "set" []),("B",mk_sort "set" [])]
+val _ = new_sort_infix "fun" "->"
+
+fun fun_sort A B = mk_sort "fun" [A,B]
+fun mk_func f A B = mk_var(f,fun_sort A B)
+val _ = EqSorts := "fun" :: (!EqSorts)
+
+val _ = new_fun "App" (mem_sort (mk_set "B"),
+                       [("f",fun_sort (mk_set "A") (mk_set "B")),
+                       ("a",mem_sort (mk_set "A"))]);
+
+val rel2fun = store_ax("rel2fun",
+“!A B R:A~>B. isFun(R) ==> ?!f:A->B. !a b. App(f,a) = b <=> Holds(R,a,b)”);
+
+val asF_def = rel2fun |> spec_all |> undisch
+                      |> uex_expand |> ex2fsym0 "asF" ["R"]
+                      |> disch_all |> gen_all
+                      |> store_as "asF_def";
+
+val asF_App = asF_def |> spec_all |> undisch |> conjE1
+                      |> disch_all |> gen_all
+                      |> store_as "asF_App";
+
+val is_asF = asF_def |> spec_all |> undisch |> conjE2
+                      |> disch_all |> gen_all
+                      |> store_as "is_asF";
+
+
+val Inj_def = define_pred
+ “!A B R:rel(A,B). isInj(R) <=> isFun(R) & !x1:mem(A) x2:mem(A). Eval(R,x1) = Eval(R,x2) ==> x1 = x2”;
+val Surj_def = define_pred “!A B R:rel(A,B). isSurj(R) <=> isFun(R) & !y:mem(B).?x:mem(A). Eval(R,x) = y”;
+val Bij_def = define_pred “!A B R:A~>B. isBij(R) <=> isInj(R) & isSurj(R)”;
+
+val INJ = define_pred 
+“!A B f:A->B.INJ(f) <=> (!a1 a2. App(f,a1) = App(f,a2) ==> a1 = a2)”;
+
+
+val SURJ = define_pred 
+“!A B f:A->B.SURJ(f) <=> (!b. ?a. App(f,a) = b)”
+
+val BIJ = define_pred
+“!A B f:A->B.BIJ(f) <=> (INJ(f) & SURJ(f))”
+
+val AX1 = new_ax
+“!A B:set.?!R:A~>B.!a:mem(A) b:mem(B).Holds(R,a,b)<=> P(a,b)”;
+
+local
+val l = fVar_Inst 
+[("P",([("a",mem_sort (mk_set "A")),("b",mem_sort (mk_set "B"))],
+ “App(f1:A->B,a) = b”))] 
+(AX1 |> qspecl [‘A’, ‘B’] |> uex_expand)
+in
+val fun_ext0 = prove_store("fun_ext0",
+e0
+(rpt strip_tac >> 
+ strip_assume_tac l >> pop_assum (K all_tac) >>
+ assume_tac rel2fun >>
+ first_x_assum (qsspecl_then [‘R’] assume_tac) >>
+ qby_tac ‘isFun(R)’ 
+ >-- (rw[Fun_expand] >> arw[] >> 
+     rpt strip_tac >-- (qexists_tac ‘App(f2,a)’ >> rw[]) >>
+     pop_assum (assume_tac o GSYM) >> arw[]) >>
+ first_x_assum drule >> 
+ pop_assum (strip_assume_tac o uex_expand) >>
+ qsuff_tac ‘f1 = f & f2 = f’ >-- (strip_tac >> arw[]) >> strip_tac (* 2 *)
+ >> (first_x_assum irule >> arw[]))
+(form_goal
+ “!A B f1:A->B f2. (!a. App(f1,a) = App(f2,a)) ==> f1 = f2”));
+end
+
+
+val fun_ext = prove_store("fun_ext",
+e0
+(rpt strip_tac >> dimp_tac >> rpt strip_tac >> arw[] >>
+ drule fun_ext0 >> arw[])
+(form_goal
+ “!A B f1:A->B f2. (!a. App(f1,a) = App(f2,a)) <=> f1 = f2”));
+
+
+
+
+local
+val l = fVar_Inst 
+[("P",([("a",mem_sort (mk_set "A")),("b",mem_sort (mk_set "B"))],
+ “App(f:A->B,a) = b”))] 
+(AX1 |> qspecl [‘A’, ‘B’] |> uex_expand)
+in
+val asR_ex = prove_store("asR_ex",
+e0
+(rpt strip_tac >> strip_assume_tac l >>
+ qexists_tac ‘R’ >> arw[])
+(form_goal
+ “!A B f:A->B.?R.!a b. Holds(R,a,b) <=> App(f,a) = b”));
+end
+
+
+val asR_def = asR_ex |> spec_all |> ex2fsym0 "asR" ["f"]
+                     |> gen_all
+
+
+val asR_Fun = prove_store("asR_Fun",
+e0
+(rpt strip_tac >> rw[Fun_expand] >>
+ rw[asR_def] >> rpt strip_tac (* 2 *)
+ >-- (qexists_tac ‘App(f,a)’ >> rw[]) >>
+ pop_assum (assume_tac o GSYM) >> arw[])
+(form_goal
+ “!A B f:A->B. isFun(asR(f))”));
+
+
+
+val _ = new_fun "@" (rel_sort (mk_set "A") (mk_set "C"),
+                     [("phi",rel_sort (mk_set "B") (mk_set "C")),
+                      ("psi",rel_sort (mk_set "A") (mk_set "B"))])
+
+
+val oR_def = new_ax 
+“!A B phi:A~>B C psi:B~>C a:mem(A) c:mem(C). 
+(?b. Holds(phi,a,b) & Holds(psi,b,c)) <=> Holds(psi @ phi,a,c)”
+
+val _ = new_fun "id" (rel_sort (mk_set "A") (mk_set "A"),
+                     [("A",set_sort)])
+
+val id_def = new_ax “!A a:mem(A) b. Holds(id(A),a,b) <=> a = b”;
+
+
+val id_Fun = prove_store("id_Fun",
+e0
+(strip_tac >> rw[Fun_expand,id_def] >> flip_tac >> rpt strip_tac >>
+ arw[] >> qexists_tac ‘a’ >> rw[])
+(form_goal
+ “!A. isFun(id(A))”));
+
+
+local
+val l = 
+ fVar_Inst 
+[("P",([("a",mem_sort (mk_set "A")),("b",mem_sort (mk_set "B"))],
+“Holds(R1:A~>B,a,b)”))] 
+(AX1 |> qspecl [‘A’,‘B’]) |> uex_expand
+in
+val R_EXT = prove_store("R_EXT",
+e0
+(rpt strip_tac >> dimp_tac >> rpt strip_tac >> arw[] >>
+ strip_assume_tac l >>
+ qsuff_tac ‘R1 = R & R2= R’ >-- (strip_tac >> arw[]) >> 
+ strip_tac >> first_x_assum irule >> arw[]
+ )
+(form_goal
+“!A B R1:A~>B R2. R1 = R2 <=> !a b.Holds(R1,a,b) <=> Holds(R2,a,b)”));
+end
+
+
+val FUN_EXT = prove_store("FUN_EXT",
+e0
+(rpt strip_tac >> drule Eval_def >> 
+ rev_drule Eval_def >> dimp_tac >> rpt strip_tac (* 2 *)
+ >-- (drule $ iffLR R_EXT >>
+      first_x_assum (qspecl_then [‘a’,‘Eval(f2,a)’] assume_tac) >>
+      rev_full_simp_tac[]) >>
+ irule $ iffRL R_EXT >> rpt strip_tac >>
+ arw[])
+(form_goal “!A B f1:A~>B f2. isFun(f1) & isFun(f2) ==>
+ (f1 = f2 <=> (!a.Eval(f1,a) = Eval(f2,a)))”));
+
+
+val idL = prove_store("idL",
+e0
+(rpt strip_tac >> irule $ iffRL R_EXT >> 
+ rw[GSYM oR_def,id_def] >> rpt strip_tac >> dimp_tac >> strip_tac
+ >-- fs[] >> qexists_tac ‘b’ >> arw[])
+(form_goal
+ “!A B f:A~>B. id(B) @ f = f”));
+
+
+val idR = prove_store("idR",
+e0
+(rpt strip_tac >> irule $ iffRL R_EXT >> 
+ rw[GSYM oR_def,id_def] >> rpt strip_tac >> dimp_tac >> strip_tac
+ >-- fs[] >> qexists_tac ‘a’ >> arw[])
+(form_goal
+ “!A B f:A~>B. f @ id(A) = f”));
+
+val Eval_id = prove_store("Eval_id",
+e0
+(rpt strip_tac >> qspecl_then [‘A’] assume_tac id_Fun >>
+ drule $ GSYM Eval_def >> flip_tac >> arw[] >> rw[id_def])
+(form_goal
+ “!A a.Eval(id(A),a) = a”));
+
+
+
+val Thm_2_7_oR_Fun = proved_th $
+e0
+(rpt strip_tac >> fs[Fun_expand,GSYM oR_def] >> rpt strip_tac (* 2 *)
+ >-- (last_x_assum (qspecl_then [‘a’] strip_assume_tac) >>
+      last_x_assum (qspecl_then [‘b’] strip_assume_tac) >>
+      qexistsl_tac [‘b'’,‘b’] >> arw[]) >>
+ first_x_assum irule >> 
+ qby_tac ‘b' = b’ >--
+ (first_x_assum irule >> qexistsl_tac [‘a’] >> arw[]) >>
+ fs[] >> qexists_tac ‘b’ >> arw[])
+(form_goal
+ “!A B f:A~>B C g:B~>C. isFun(f) & isFun(g) ==> isFun(g @ f)”)
+
+val oR_Fun = Thm_2_7_oR_Fun |> store_as "oR_Fun"
+
+val o_ex = prove_store("o_ex",
+e0
+(rpt strip_tac >>
+ qexists_tac ‘asF(asR(psi) @ asR(phi))’ >> 
+ qsspecl_then [‘psi’] assume_tac asR_Fun >>
+ qsspecl_then [‘phi’] assume_tac asR_Fun >>
+ qby_tac ‘isFun(asR(psi) @ asR(phi))’ 
+ >-- (irule oR_Fun >> arw[]) >>
+ drule asF_App >> arw[])
+(form_goal
+ “!A B phi:A->B C psi:B->C. ?f:A->C. 
+ !a c. App(f,a) = c <=> Holds(asR(psi) @ asR(phi),a,c)”));
+
+val o_def = o_ex |> spec_all |> ex2fsym0 "o" ["psi","phi"]
+                 |> gen_all |> store_as "o_def";
+
+val o_App = prove_store("o_App",
+e0
+(rpt strip_tac >> flip_tac >> rw[o_def] >>
+ rw[GSYM oR_def] >>
+ qexists_tac ‘App(f,a)’ >> rw[asR_def])
+(form_goal
+ “!A B f:A->B C g:B->C a. App(g,(App(f,a))) = App(g o f,a)”));
+
+
+val asR_oR = prove_store("asR_oR",
+e0
+(rpt strip_tac >> irule $ iffRL R_EXT >> rpt strip_tac >>
+ rw[asR_def] >> rw[o_def])
+(form_goal
+ “!A B f:A->B C g:B-> C. asR(g) @ asR(f) = asR(g o f)”));
+
+
+val asR_asF = prove_store("asR_asF",
+e0
+(rpt strip_tac >> irule $ iffRL R_EXT >>
+ rw[asR_def] >> drule asF_App >> arw[])
+(form_goal
+ “!A B f:A~>B. isFun(f) ==> asR(asF(f)) =f”));
+
+
+
+(*Thm_2_3_5*)
+val To1_fun_uex = prove_store("To1_fun_uex",
+e0
+(strip_tac >> uex_tac >> qexists_tac ‘asF(To1(A))’ >> rw[] >>
+ strip_tac >> irule is_asF >> rw[To1_Fun] >> rw[dot_def] >>
+ rpt strip_tac >> 
+ qspecl_then [‘A’] assume_tac To1_Fun >>
+ drule Eval_def >> arw[dot_def]
+ )
+(form_goal
+ “!A. ?!f:A~>1. T”));
